src/study/Nemonuri.Study.CSharpSyntaxRewriter2.Modifier2/Nemonuri.StratifiedNodes.Forall.Children.fst
@@ -1,0 +1,51 @@
+module Nemonuri.StratifiedNodes.Forall.Children
+
+module L = FStar.List.Tot
+module N = Nemonuri.StratifiedNodes.Nodes
+module C = Nemonuri.StratifiedNodes.Children
+module Common = Nemonuri.StratifiedNodes.Common
+module D = Nemonuri.StratifiedNodes.Decreasers
+module F = Nemonuri.StratifiedNodes.Factories
+
+//--- theory members ---
+
+let for_all_aggregator
+  : (Common.aggregator bool) =
+  fun v1 v2 -> (v1 && v2)
+
+let for_all_continue_predicate (t:eqtype)
+  : (C.continue_predicate t bool) 
+  =
+  fun n v -> v
+
+(*
+let for_all_select_and_aggregate_from_children_internal #t (parent:N.node t) 
+  (parent_value: t2)
+  (node_predicate:N.node t -> Tot bool)
+*)
+
+let for_all_select_and_aggregate_from_children #t
+  (parent:N.node t) 
+  (node_predicate:N.node t -> Tot bool)
+  (ancestors:C.head_given_ancestor_list parent)
+  : Tot bool =
+  let selector : (C.ancestor_list_given_selector_for_child t bool parent) = (
+    C.to_ancestor_list_given_selector_for_child t bool
+      parent node_predicate
+  ) in
+  let parent_value = node_predicate parent in
+  C.select_and_aggregate_from_children 
+    parent parent_value selector
+    for_all_aggregator
+    for_all_aggregator
+    (Common.aggregated_identity bool)
+    (for_all_continue_predicate t)
+    ancestors
+
+//---|
+
+//--- propositions ---
+//---|
+
+//--- proof ---
+//---|
